<?xml version="1.0"?>
<rdf:RDF 
    xmlns:dcterms="http://purl.org/dc/terms/"
    xmlns:ldp="http://www.w3.org/ns/ldp#"
    xmlns:ore="http://www.openarchives.org/ore/terms/"
    xmlns:owl="http://www.w3.org/2002/07/owl#"
    xmlns:rdf="http://www.w3.org/1999/02/22-rdf-syntax-ns#"
    xmlns:rdfs="http://www.w3.org/2000/01/rdf-schema#"
    xmlns:xsd="http://www.w3.org/2001/XMLSchema#">

    <rdf:Description rdf:about="http://pcdm.org/models#">
      <dcterms:title xml:lang="en">Portland Common Data Model</dcterms:title>
      <dcterms:modified rdf:datatype="http://www.w3.org/2001/XMLSchema#date">2015-03-16</dcterms:modified>
      <dcterms:publisher rdf:resource="http://www.duraspace.org/"/>
      <rdfs:seeAlso rdf:resource="https://wiki.duraspace.org/display/FF/Portland+Common+Data+Model"/>
      <rdfs:comment xml:lang="en">Ontology for the Portland Common Data Model, intended to underlie a wide array of repository and DAMS applications.</rdfs:comment>
      <owl:versionInfo>2015/03/16</owl:versionInfo>
    </rdf:Description>
    
    <rdfs:Class rdf:about="http://pcdm.org/models#AdministrativeSet">
      <rdfs:label xml:lang="en">Administrative Set</rdfs:label>
      <rdfs:comment xml:lang="en">
        An Administrative Set is a grouping of resources that an administrative unit is ultimately
        responsible for managing. The set itself helps to manage the items within it. An Object
        or Collection may be contained by only one AdministrativeSet.
      </rdfs:comment>
      <rdfs:subClassOf rdf:resource="http://www.w3.org/ns/ldp#Container"/>
      <rdfs:isDefinedBy rdf:resource="http://pcdm.org/models#"/>
    </rdfs:Class>

    <rdfs:Class rdf:about="http://pcdm.org/models#Collection">
      <rdfs:label xml:lang="en">Collection</rdfs:label>
      <rdfs:comment xml:lang="en">
        A Collection is a group of resources. Collections have descriptive metadata, access metadata,
        and may links to works and/or collections. By default, member works and collections are an
        unordered set, but can be ordered using the ORE Proxy class.
      </rdfs:comment>
      <rdfs:subClassOf rdf:resource="http://www.openarchives.org/ore/terms/Aggregation"/>
      <rdfs:isDefinedBy rdf:resource="http://pcdm.org/models#"/>
    </rdfs:Class>

    <rdfs:Class rdf:about="http://pcdm.org/models#Object">
      <rdfs:label xml:lang="en">Object</rdfs:label>
      <rdfs:comment xml:lang="en">
        An Object is an intellectual entity, sometimes called a "work", "digital object", etc.
        Objects have descriptive metadata, access metadata, may contain files and other Objects as
        member "components". Each level of a work is therefore represented by an Object instance,
        and is capable of standing on its own, being linked to from Collections and other Objects.
        Member Objects can be ordered using the ORE Proxy class.
      </rdfs:comment>
      <rdfs:subClassOf rdf:resource="http://www.openarchives.org/ore/terms/Aggregation"/>
      <rdfs:isDefinedBy rdf:resource="http://pcdm.org/models#"/>
    </rdfs:Class>
   
    <rdfs:Class rdf:about="http://pcdm.org/models#File">
      <rdfs:label xml:lang="en">File</rdfs:label>
      <rdfs:comment xml:lang="en">
        A File is a sequence of binary data and is described by some accompanying metadata.
        The metadata typically includes at least basic technical metadata (size, content type,
        modification date, etc.), but can also include properties related to preservation,
        digitization process, provenance, etc. Files MUST be contained by exactly one Object.
      </rdfs:comment>
      <rdfs:isDefinedBy rdf:resource="http://pcdm.org/models#"/>
    </rdfs:Class>

    <rdf:Property rdf:about="http://pcdm.org/models#hasFile">
      <rdfs:label xml:lang="en">has file</rdfs:label>
      <rdfs:comment xml:lang="en">Links to a File contained by this Object.</rdfs:comment>
      <rdfs:domain rdf:resource="http://pcdm.org/models#Object"/>
      <rdfs:range rdf:resource="http://pcdm.org/models#File"/>
      <rdfs:subPropertyOf rdf:resource="http://www.w3.org/ns/ldp#contains"/>
      <rdfs:isDefinedBy rdf:resource="http://pcdm.org/models#"/>
    </rdf:Property>

    <rdf:Property rdf:about="http://pcdm.org/models#hasMember">
      <rdfs:label xml:lang="en">has member</rdfs:label>
      <rdfs:comment xml:lang="en">Links to a related Object. Typically used to link to component parts, such as a book linking to a page.</rdfs:comment>
      <rdfs:domain rdf:resource="http://www.openarchives.org/ore/terms/Aggregation"/>
      <rdfs:range rdf:resource="http://www.openarchives.org/ore/terms/Aggregation"/>
      <rdfs:subPropertyOf rdf:resource="http://www.openarchives.org/ore/terms/aggregates"/>
      <rdfs:isDefinedBy rdf:resource="http://pcdm.org/models#"/>
    </rdf:Property>

    <rdf:Property rdf:about="http://pcdm.org/models#hasRelatedFile">
      <rdfs:label xml:lang="en">has related file</rdfs:label>
      <rdfs:comment xml:lang="en">Links to a File which is related to this Object but doesn't directly describe or represent it, such as technical metadata about other files.</rdfs:comment>
      <rdfs:domain rdf:resource="http://pcdm.org/models#Object"/>
      <rdfs:range rdf:resource="http://pcdm.org/models#File"/>
      <rdfs:subPropertyOf rdf:resource="http://www.w3.org/ns/ldp#contains"/>
      <rdfs:isDefinedBy rdf:resource="http://pcdm.org/models#"/>
    </rdf:Property>
    
    <rdf:Property rdf:about="http://pcdm.org/models#hasRelatedObject">
      <rdfs:label xml:lang="en">has related object</rdfs:label>
      <rdfs:comment xml:lang="en">Links to an Object which is related to this Object but doesn't directly describe or represent it.</rdfs:comment>
      <rdfs:domain rdf:resource="http://pcdm.org/models#Object"/>
      <rdfs:domain rdf:resource="http://pcdm.org/models#Collection"/>
      <rdfs:range rdf:resource="http://pcdm.org/models#Object"/>
      <rdfs:subPropertyOf rdf:resource="http://purl.org/dc/elements/1.1/relation"/>
      <rdfs:isDefinedBy rdf:resource="http://pcdm.org/models#"/>
    </rdf:Property>
</rdf:RDF>
