<?xml version="1.0"?>
<?xml-stylesheet type="text/xsl" href="rdfs2html.xsl"?>
<rdf:RDF 
    xmlns:dcterms="http://purl.org/dc/terms/"
    xmlns:ldp="http://www.w3.org/ns/ldp#"
    xmlns:ore="http://www.openarchives.org/ore/terms/"
    xmlns:owl="http://www.w3.org/2002/07/owl#"
    xmlns:rdf="http://www.w3.org/1999/02/22-rdf-syntax-ns#"
    xmlns:rdfs="http://www.w3.org/2000/01/rdf-schema#"
    xmlns:xsd="http://www.w3.org/2001/XMLSchema#"
    xmlns:pcdm="http://pcdm.org/models#">

    <rdf:Description rdf:about="http://pcdm.org/models#">
      <dcterms:title xml:lang="en">Portland Common Data Model</dcterms:title>
      <dcterms:modified rdf:datatype="http://www.w3.org/2001/XMLSchema#date">2015-10-14</dcterms:modified>
      <dcterms:publisher rdf:resource="http://www.duraspace.org/"/>
      <rdfs:seeAlso rdf:resource="https://github.com/duraspace/pcdm/wiki"/>
      <rdfs:comment xml:lang="en">Ontology for the Portland Common Data Model, intended to underlie a wide array of repository and DAMS applications.</rdfs:comment>
      <owl:versionInfo>2016/04/18</owl:versionInfo>
      <owl:priorVersion rdf:resource="http://pcdm.org/2015/04/18/models"/>
    </rdf:Description>
    
    <rdfs:Class rdf:about="http://pcdm.org/models#Collection">
      <rdfs:label xml:lang="en">Collection</rdfs:label>
      <rdfs:comment xml:lang="en">
        A Collection is a group of resources. Collections have descriptive metadata, access metadata,
        and may links to works and/or collections. By default, member works and collections are an
        unordered set, but can be ordered using the ORE Proxy class.
      </rdfs:comment>
      <rdfs:subClassOf rdf:resource="http://www.openarchives.org/ore/terms/Aggregation"/>
      <rdfs:isDefinedBy rdf:resource="http://pcdm.org/models#"/>
    </rdfs:Class>

    <rdfs:Class rdf:about="http://pcdm.org/models#Object">
      <rdfs:label xml:lang="en">Object</rdfs:label>
      <rdfs:comment xml:lang="en">
        An Object is an intellectual entity, sometimes called a "work", "digital object", etc.
        Objects have descriptive metadata, access metadata, may contain files and other Objects as
        member "components". Each level of a work is therefore represented by an Object instance,
        and is capable of standing on its own, being linked to from Collections and other Objects.
        Member Objects can be ordered using the ORE Proxy class.
      </rdfs:comment>
      <rdfs:subClassOf rdf:resource="http://www.openarchives.org/ore/terms/Aggregation"/>
      <rdfs:isDefinedBy rdf:resource="http://pcdm.org/models#"/>
    </rdfs:Class>
   
    <rdfs:Class rdf:about="http://pcdm.org/models#AlternateOrder">
      <rdfs:label xml:lang="en">Alternate Order</rdfs:label>
      <rdfs:comment xml:lang="en">
        An AlternateOrder is an alternate ordering of its parent's members.  It should only order the
        parent's members, and otherwise has all of the features of ordering (some members may be
        omitted from the order, members may appear more than once in the order, etc.).
      </rdfs:comment>
      <rdfs:subClassOf rdf:resource="http://pcdm.org/models#Object"/>
      <rdfs:isDefinedBy rdf:resource="http://pcdm.org/models#"/>
    </rdfs:Class>

    <rdfs:Class rdf:about="http://pcdm.org/models#File">
      <rdfs:label xml:lang="en">File</rdfs:label>
      <rdfs:comment xml:lang="en">
        A File is a sequence of binary data and is described by some accompanying metadata.
        The metadata typically includes at least basic technical metadata (size, content type,
        modification date, etc.), but can also include properties related to preservation,
        digitization process, provenance, etc. Files MUST be contained by exactly one Object.
      </rdfs:comment>
      <rdfs:isDefinedBy rdf:resource="http://pcdm.org/models#"/>
    </rdfs:Class>

    <rdf:Property rdf:about="http://pcdm.org/models#hasFile">
      <rdfs:label xml:lang="en">has file</rdfs:label>
      <rdfs:comment xml:lang="en">Links to a File contained by this Object.</rdfs:comment>
      <rdfs:domain rdf:resource="http://pcdm.org/models#Object"/>
      <rdfs:range rdf:resource="http://pcdm.org/models#File"/>
      <rdfs:subPropertyOf rdf:resource="http://www.openarchives.org/ore/terms/aggregates"/>
      <rdfs:isDefinedBy rdf:resource="http://pcdm.org/models#"/>
    </rdf:Property>

    <rdf:Property rdf:about="http://pcdm.org/models#fileOf">
      <rdfs:label xml:lang="en">is file of</rdfs:label>
      <rdfs:comment xml:lang="en">Links from a File to its containing Object.</rdfs:comment>
      <rdfs:range rdf:resource="http://pcdm.org/models#Object"/>
      <rdfs:domain rdf:resource="http://pcdm.org/models#File"/>
      <rdfs:subPropertyOf rdf:resource="http://www.openarchives.org/ore/terms/isAggregatedBy"/>
      <rdfs:isDefinedBy rdf:resource="http://pcdm.org/models#"/>
      <owl:inverseOf rdf:resource="http://pcdm.org/models#hasFile"/>
    </rdf:Property>

    <rdf:Property rdf:about="http://pcdm.org/models#hasMember">
      <rdfs:label xml:lang="en">has member</rdfs:label>
      <rdfs:comment xml:lang="en">Links to a subsidiary Object or Collection. Typically used to link
          to component parts, such as a book linking to a page.  Note on transitivity: hasMember is
          not defined as transitive, but applications may treat it as transitive as local needs
          dictate.</rdfs:comment>
      <rdfs:domain rdf:resource="http://www.openarchives.org/ore/terms/Aggregation"/>
      <rdfs:range rdf:resource="http://www.openarchives.org/ore/terms/Aggregation"/>
      <rdfs:subPropertyOf rdf:resource="http://www.openarchives.org/ore/terms/aggregates"/>
      <rdfs:isDefinedBy rdf:resource="http://pcdm.org/models#"/>
    </rdf:Property>

    <rdf:Property rdf:about="http://pcdm.org/models#memberOf">
      <rdfs:label xml:lang="en">is member of</rdfs:label>
      <rdfs:comment xml:lang="en">Links from an Object or Collection to a containing Object or Collection.</rdfs:comment>
      <rdfs:range rdf:resource="http://www.openarchives.org/ore/terms/Aggregation"/>
      <rdfs:domain rdf:resource="http://www.openarchives.org/ore/terms/Aggregation"/>
      <rdfs:subPropertyOf rdf:resource="http://www.openarchives.org/ore/terms/isAggregatedBy"/>
      <rdfs:isDefinedBy rdf:resource="http://pcdm.org/models#"/>
      <owl:inverseOf rdf:resource="http://pcdm.org/models#hasMember"/>
    </rdf:Property>

    <rdf:Property rdf:about="http://pcdm.org/models#hasRelatedObject">
      <rdfs:label xml:lang="en">has related object</rdfs:label>
      <rdfs:comment xml:lang="en">Links to a related Object that is not a component part, such as an object representing a donor agreement or policies that govern the resource.</rdfs:comment>
      <rdfs:domain rdf:resource="http://www.openarchives.org/ore/terms/Aggregation"/>
      <rdfs:range rdf:resource="http://pcdm.org/models#Object"/>
      <rdfs:subPropertyOf rdf:resource="http://www.openarchives.org/ore/terms/aggregates"/>
      <rdfs:isDefinedBy rdf:resource="http://pcdm.org/models#"/>
    </rdf:Property>

    <rdf:Property rdf:about="http://pcdm.org/models#relatedObjectOf">
      <rdfs:label xml:lang="en">is related object of</rdfs:label>
      <rdfs:comment xml:lang="en">Links from an Object to a Object or Collection that it is related to.</rdfs:comment>
      <rdfs:range rdf:resource="http://www.openarchives.org/ore/terms/Aggregation"/>
      <rdfs:domain rdf:resource="http://pcdm.org/models#Object"/>
      <rdfs:subPropertyOf rdf:resource="http://www.openarchives.org/ore/terms/isAggregatedBy"/>
      <rdfs:isDefinedBy rdf:resource="http://pcdm.org/models#"/>
      <owl:inverseOf rdf:resource="http://pcdm.org/models#hasRelatedObject"/>
    </rdf:Property>
   
</rdf:RDF>
