<?xml version="1.0"?>
<rdf:RDF
    xmlns:dcterms="http://purl.org/dc/terms/"
    xmlns:owl="http://www.w3.org/2002/07/owl#"
    xmlns:rdf="http://www.w3.org/1999/02/22-rdf-syntax-ns#"
    xmlns:rdfs="http://www.w3.org/2000/01/rdf-schema#">

  <rdf:Description rdf:about="http://pcdm.org/rights#">
    <dcterms:title xml:lang="en">Portland Common Data Model: Rights Extension</dcterms:title>
    <dcterms:modified rdf:datatype="http://www.w3.org/2001/XMLSchema#date">2015-06-03</dcterms:modified>
    <dcterms:publisher rdf:resource="http://www.duraspace.org/"/>
    <rdfs:seeAlso rdf:resource="https://github.com/duraspace/pcdm/wiki"/>
    <rdfs:seeAlso rdf:resource="https://wiki.duraspace.org/display/hydra/Rights+Metadata+Subgroup"/>
    <rdfs:comment xml:lang="en">Ontology for a PCDM extension to add properties for rights
        overrides.</rdfs:comment>
    <owl:versionInfo>2015/06/03</owl:versionInfo>
  </rdf:Description>

    <rdf:Property rdf:about="http://pcdm.org/rights#rightsOverride">
      <rdfs:label xml:lang="en">rights override</rdfs:label>
      <rdfs:comment xml:lang="en">Links to a rights statement that overrides the base rights statement
          attached to a resource.  This could be an embargo, temporary license, statutory
          restriction.</rdfs:comment>
      <rdfs:range rdf:resource="http://purl.org/dc/terms/RightsStatement"/>
      <rdfs:subPropertyOf rdf:resource="http://purl.org/dc/terms/accessRights"/>
      <rdfs:isDefinedBy rdf:resource="http://pcdm.org/rights#"/>
    </rdf:Property>

    <rdf:Property rdf:about="http://pcdm.org/rights#rightsOverrideExpiration">
      <rdfs:label xml:lang="en">rights override expiration</rdfs:label>
      <rdfs:comment xml:lang="en">Date when a rights override expires.  After this date, the base rights
          rights statement will be in effect.  Recommended best practice is to use an encoding scheme,
          such as the W3CDTF profile of ISO 8601.</rdfs:comment>
      <rdfs:range rdf:resource="http://www.w3.org/2000/01/rdf-schema#Literal"/>
      <rdfs:subPropertyOf rdf:resource="http://purl.org/dc/terms/date"/>
      <rdfs:isDefinedBy rdf:resource="http://pcdm.org/rights#"/>
    </rdf:Property>

</rdf:RDF>
