<?xml version="1.0"?>
<?xml-stylesheet type="text/xsl" href="rdfs2html.xsl"?>
<rdf:RDF
    xmlns:dcterms="http://purl.org/dc/terms/"
    xmlns:owl="http://www.w3.org/2002/07/owl#"
    xmlns:rdf="http://www.w3.org/1999/02/22-rdf-syntax-ns#"
    xmlns:rdfs="http://www.w3.org/2000/01/rdf-schema#">

  <rdf:Description rdf:about="http://pcdm.org/use#">
    <dcterms:title xml:lang="en">Portland Common Data Model: Use Extension</dcterms:title>
    <dcterms:modified rdf:datatype="http://www.w3.org/2001/XMLSchema#date">2015-05-12</dcterms:modified>
    <dcterms:publisher rdf:resource="http://www.duraspace.org/"/>
    <rdfs:seeAlso rdf:resource="https://github.com/duraspace/pcdm/wiki"/>
    <rdfs:seeAlso rdf:resource="https://wiki.duraspace.org/display/hydra/File+Use+Vocabulary"/>
    <rdfs:comment xml:lang="en">Ontology for a PCDM extension to add subclasses of PCDM File for the
        different roles files have in relation to the Object they are attached to.</rdfs:comment>
    <owl:versionInfo>2021/04/09</owl:versionInfo>
    <owl:priorVersion rdf:resource="http://pcdm.org/2015/05/12/use"/>
  </rdf:Description>

  <rdfs:Class rdf:about="http://pcdm.org/use#ExtractedText">
    <rdfs:label xml:lang="en">extracted text</rdfs:label>
    <rdfs:comment xml:lang="en">A textual representation of the Object appropriate for fulltext indexing,
        such as a plaintext version of a document, or OCR text.</rdfs:comment>
    <rdf:subClassOf rdf:resource="http://pcdm.org/models#File"/>
    <rdfs:isDefinedBy rdf:resource="http://pcdm.org/use#"/>
  </rdfs:Class>

  <rdfs:Class rdf:about="http://pcdm.org/use#IntermediateFile">
    <rdfs:label xml:lang="en">intermediate file</rdfs:label>
    <rdfs:comment xml:lang="en">High quality representation of the Object, appropriate for generating
        derivatives or other additional processing.</rdfs:comment>
    <rdf:subClassOf rdf:resource="http://pcdm.org/models#File"/>
    <rdfs:isDefinedBy rdf:resource="http://pcdm.org/use#"/>
  </rdfs:Class>

  <rdfs:Class rdf:about="http://pcdm.org/use#OriginalFile">
    <rdfs:label xml:lang="en">original file</rdfs:label>
    <rdfs:comment xml:lang="en">The original creation format of a file.</rdfs:comment>
    <rdf:subClassOf rdf:resource="http://pcdm.org/models#File"/>
    <rdfs:isDefinedBy rdf:resource="http://pcdm.org/use#"/>
  </rdfs:Class>

  <rdfs:Class rdf:about="http://pcdm.org/use#PreservationFile">
    <rdfs:label xml:lang="en">preservation file</rdfs:label>
    <rdfs:comment xml:lang="en">Best quality representation of the Object appropriate for long-term
        preservation.</rdfs:comment>
    <rdf:subClassOf rdf:resource="http://pcdm.org/models#File"/>
    <dcterms:replaces rdf:resource="http://pcdm.org/use#PreservationMasterFile"/>
    <rdfs:isDefinedBy rdf:resource="http://pcdm.org/use#"/>
  </rdfs:Class>

  <rdfs:Class rdf:about="http://pcdm.org/use#PreservationMasterFile">
    <rdfs:label xml:lang="en">preservation master file</rdfs:label>
    <rdfs:comment xml:lang="en">Best quality representation of the Object appropriate for long-term
        preservation.</rdfs:comment>
    <rdfs:comment>Note: This class has been deprecated in favor of PreservationFile.</rdfs:comment>
    <rdf:subClassOf rdf:resource="http://pcdm.org/models#File"/>
    <dcterms:isReplacedBy rdf:resource="http://pcdm.org/use#PreservationFile"/>
    <owl:deprecated rdf:datatype="http://www.w3.org/2001/XMLSchema#boolean">true</owl:deprecated>
    <rdfs:isDefinedBy rdf:resource="http://pcdm.org/use#"/>
  </rdfs:Class>

  <rdfs:Class rdf:about="http://pcdm.org/use#ServiceFile">
    <rdfs:label xml:lang="en">service file</rdfs:label>
    <rdfs:comment xml:lang="en">A medium quality representation of the Object appropriate for serving to
        users.  Similar to a FADGI "derivative file" but can also be used for born-digital content,
        and is not necessarily derived from another file.</rdfs:comment>
    <rdf:subClassOf rdf:resource="http://pcdm.org/models#File"/>
    <rdfs:isDefinedBy rdf:resource="http://pcdm.org/use#"/>
  </rdfs:Class>

  <rdfs:Class rdf:about="http://pcdm.org/use#ThumbnailImage">
    <rdfs:label xml:lang="en">thumbnail image</rdfs:label>
    <rdfs:comment xml:lang="en">A low resolution image representation of the Object appropriate for using
        as an icon.</rdfs:comment>
    <rdf:subClassOf rdf:resource="http://pcdm.org/models#File"/>
    <rdfs:isDefinedBy rdf:resource="http://pcdm.org/use#"/>
  </rdfs:Class>

  <rdfs:Class rdf:about="http://pcdm.org/use#Transcript">
    <rdfs:label xml:lang="en">transcript</rdfs:label>
    <rdfs:comment xml:lang="en">A textual representation of the Object appropriate for presenting to users,
        such as subtitles or transcript of a video.  Can be used as a substitute or complement to other
        files for accessibility purposes.</rdfs:comment>
    <rdf:subClassOf rdf:resource="http://pcdm.org/models#ExtractedText"/>
    <rdfs:isDefinedBy rdf:resource="http://pcdm.org/use#"/>
  </rdfs:Class>

</rdf:RDF>
