<?xml version="1.0"?>
<?xml-stylesheet type="text/xsl" href="rdfs2html.xsl"?>
<rdf:RDF
    xmlns:dcterms="http://purl.org/dc/terms/"
    xmlns:owl="http://www.w3.org/2002/07/owl#"
    xmlns:rdf="http://www.w3.org/1999/02/22-rdf-syntax-ns#"
    xmlns:rdfs="http://www.w3.org/2000/01/rdf-schema#"
    xmlns:skos="http://www.w3.org/2004/02/skos/core#">

  <rdf:Description rdf:about="http://pcdm.org/works#">
    <dcterms:title xml:lang="en">Portland Common Data Model: Works Extension</dcterms:title>
    <dcterms:modified rdf:datatype="http://www.w3.org/2001/XMLSchema#date">2021-04-09</dcterms:modified>
    <dcterms:publisher rdf:resource="http://www.duraspace.org/"/>
    <rdfs:seeAlso rdf:resource="https://github.com/duraspace/pcdm/wiki"/>
    <rdfs:seeAlso rdf:resource="http://iiif.io/api/presentation/2.0/"/>
    <rdfs:comment xml:lang="en">Ontology for a PCDM extension that adds subclasses of pcdm:Object
      to refine the relationships between a work and its constituent parts.  Also establishes
      links to the IIIF Presentation API.</rdfs:comment>
    <owl:versionInfo>2021/04/09</owl:versionInfo>
    <owl:priorVersion rdf:resource="http://pcdm.org/2016/02/16/works"/>
  </rdf:Description>

  <rdfs:Class rdf:about="http://pcdm.org/works#Work">
    <rdfs:label xml:lang="en">Work</rdfs:label>
    <rdfs:comment xml:lang="en">
      A work or intellectual entity, such as a book, film, dissertation, etc.
      Works have member Objects representing their physical structure (e.g., pages in a book),
      FileSets to maintain representations of the entire resource (e.g. a PDF of all the pages),
      and TopRanges representing their logical structure or structures (e.g., sections
      and chapters in a book).
    </rdfs:comment>
    <rdfs:subClassOf rdf:resource="http://pcdm.org/models#Object"/>
    <rdfs:isDefinedBy rdf:resource="http://pcdm.org/works#"/>
  </rdfs:Class>

  <rdfs:Class rdf:about="http://pcdm.org/works#FileSet">
    <rdfs:label xml:lang="en">FileSet</rdfs:label>
    <rdfs:comment xml:lang="en">
      A group of related Files, typically a single source File and any derivatives.
    </rdfs:comment>
    <rdfs:subClassOf rdf:resource="http://pcdm.org/models#Object"/>
    <rdfs:isDefinedBy rdf:resource="http://pcdm.org/works#"/>
  </rdfs:Class>

  <rdfs:Class rdf:about="http://pcdm.org/works#TopRange">
    <rdfs:label xml:lang="en">TopRange</rdfs:label>
    <rdfs:comment xml:lang="en">
      A logical ordering of the component parts of a Work, corresponding to a IIIF Range with
      the "top" viewing hint.  Has member Ranges that represent the logical structure, such
      as chapters within a book, scenes in a film, etc.
    </rdfs:comment>
    <skos:closeMatch rdf:resource="http://iiif.io/model/shared-canvas/1.0/#Range"/>
    <rdfs:subClassOf rdf:resource="http://pcdm.org/models#Object"/>
    <rdfs:isDefinedBy rdf:resource="http://pcdm.org/works#"/>
  </rdfs:Class>

  <rdfs:Class rdf:about="http://pcdm.org/works#Range">
    <rdfs:label xml:lang="en">Range</rdfs:label>
    <rdfs:comment xml:lang="en">
      A section of a Work, corresponding to a IIIF Range.  Has member FileSets representing the
      physical parts of the Work are part of the section (e.g., which pages are in a chapter).
    </rdfs:comment>
    <skos:closeMatch rdf:resource="http://iiif.io/model/shared-canvas/1.0/#Range"/>
    <rdfs:subClassOf rdf:resource="http://pcdm.org/models#Object"/>
    <rdfs:isDefinedBy rdf:resource="http://pcdm.org/works#"/>
  </rdfs:Class>

</rdf:RDF>
